Refactor of Result theory file to closer match rust documentation. Method names corrected where applicable. Addition of subsections to better organise the result methods.

Micro_Rust_Std_Lib/StdLib_Result.thy
@@ -8,226 +8,20 @@ begin
 (*>*)
 
 section\<open>Core material related to the \<^emph>\<open>Result\<close> type\<close>
+text\<open>Methods for Result enum as part of std::result implemented here 
+based on documentation at https://doc.rust-lang.org/std/result/enum.Result.html\<close>
 
-text\<open>Returns \<^verbatim>\<open>x\<close> if the element of \<^verbatim>\<open>Result\<close> type is of the form \<^verbatim>\<open>Ok x\<close>.  Panics otherwise with
-the defined error message.\<close>
-definition result_expect :: \<open>('v,'e) result \<Rightarrow> String.literal \<Rightarrow> ('s, 'v, 'abort, 'i, 'o) function_body\<close> where
-  \<open>result_expect self msg \<equiv> FunctionBody \<lbrakk>
-      match self {
-        Ok(v) \<Rightarrow> v,
-        Err(_) \<Rightarrow> panic!(msg) 
-      }
-  \<rbrakk>\<close>
-adhoc_overloading expect \<rightleftharpoons> result_expect
+subsection\<open>and\<close>
 
-definition result_expect_contract :: 
-  \<open>('a, 'e) result \<Rightarrow> 'a \<Rightarrow> ('s::{sepalg}, 'a, 'abort) function_contract\<close>
-  where [crush_contracts]: \<open>result_expect_contract self v \<equiv>
-    let pre = \<langle>self = Ok v\<rangle>; post = \<lambda>r. \<langle>r = v\<rangle>
-    in make_function_contract pre post\<close>
-ucincl_auto result_expect_contract
+subsection\<open>and_then\<close>
 
-lemma result_expect_spec [crush_specs]:
-  shows \<open>\<Gamma>; result_expect res m \<Turnstile>\<^sub>F result_expect_contract res v\<close>
-  by (crush_boot f: result_expect_def contract: result_expect_contract_def)
-     (crush_base split!: result.splits)
+subsection\<open>as_deref\<close>
 
-text\<open>Returns \<^verbatim>\<open>x\<close> if the element of \<^verbatim>\<open>Result\<close> type is of the form \<^verbatim>\<open>Ok x\<close>.  Panics otherwise.\<close>
-definition result_unwrap :: \<open>('v,'e) result \<Rightarrow> ('s, 'v, 'abort, 'i, 'o) function_body\<close> where
-  \<open>result_unwrap self \<equiv> FunctionBody \<lbrakk>
-      self.expect("result_unwrap")
-  \<rbrakk>\<close>
-adhoc_overloading unwrap \<rightleftharpoons> result_unwrap
+subsection\<open>as_deref_mut\<close>
 
-definition result_unwrap_contract :: 
-  \<open>('a, 'e) result \<Rightarrow> 'a \<Rightarrow> ('s::{sepalg}, 'a, 'abort) function_contract\<close>
-  where [crush_contracts]: \<open>result_unwrap_contract self v \<equiv>
-    let pre = \<langle>self = Ok v\<rangle>; post = \<lambda>r. \<langle>r = v\<rangle>
-    in make_function_contract pre post\<close>
-ucincl_auto result_unwrap_contract
+subsection\<open>as_mut\<close>
 
-lemma result_unwrap_spec [crush_specs]:
-  shows \<open>\<Gamma>; result_unwrap res \<Turnstile>\<^sub>F result_unwrap_contract res v\<close>
-  by (crush_boot f: result_unwrap_def contract: result_unwrap_contract_def)
-     (crush_base split!: result.splits)
-
-text\<open>Tests whether an element of \<^verbatim>\<open>Result\<close> type is the \<^verbatim>\<open>Err\<close> constructor:\<close>
-definition urust_func_result_is_err :: \<open>('v,'e) result \<Rightarrow> ('s, bool, 'abort, 'i, 'o) function_body\<close> where
-  \<open>urust_func_result_is_err self \<equiv> FunctionBody \<lbrakk>
-     match self {
-       Ok(_) \<Rightarrow> False,
-       Err(_) \<Rightarrow> True
-     }
-  \<rbrakk>\<close>
-
-definition result_is_err_contract :: 
-  \<open>('a, 'e) result \<Rightarrow> ('s::{sepalg}, bool, 'abort) function_contract\<close>
-  where [crush_contracts]: \<open>result_is_err_contract res \<equiv>
-    let pre = UNIV; post = \<lambda>r. \<langle>r = result_is_err res\<rangle>
-    in make_function_contract pre post\<close>
-ucincl_auto result_is_err_contract
-
-lemma result_is_err_spec [crush_specs]:
-  shows \<open>\<Gamma>; urust_func_result_is_err res \<Turnstile>\<^sub>F result_is_err_contract res\<close>
-  by (crush_boot f: urust_func_result_is_err_def contract: result_is_err_contract_def)
-     (crush_base simp add: result_is_err_def split!: result.splits)
-
-text\<open>Tests whether an element of \<^verbatim>\<open>Result\<close> type is the \<^verbatim>\<open>Ok\<close> constructor:\<close>
-definition urust_func_result_is_ok :: \<open>('v,'e) result \<Rightarrow> ('s, bool, 'abort, 'i, 'o) function_body\<close> where
-  \<open>urust_func_result_is_ok self \<equiv> FunctionBody \<lbrakk>
-     match self {
-       Ok(_) \<Rightarrow> True,
-       Err(_) \<Rightarrow> False
-     }
-  \<rbrakk>\<close>
-
-definition result_is_ok_contract :: 
-  \<open>('a, 'e) result \<Rightarrow> ('s::{sepalg}, bool, 'abort) function_contract\<close>
-  where [crush_contracts]: \<open>result_is_ok_contract res \<equiv>
-    let pre = UNIV; post = \<lambda>r. \<langle>r = result_is_ok res\<rangle>
-    in make_function_contract pre post\<close>
-ucincl_auto result_is_ok_contract
-
-lemma result_is_ok_spec [crush_specs]:
-  shows \<open>\<Gamma>; urust_func_result_is_ok res \<Turnstile>\<^sub>F result_is_ok_contract res\<close>
-  by (crush_boot f: urust_func_result_is_ok_def contract: result_is_ok_contract_def)
-     (crush_base simp add: result_is_ok_def split!: result.splits)
-
-text\<open>Returns first argument of type \<^verbatim>\<open>Result\<close> if it is the \<^verbatim>\<open>Ok\<close> constructor, returns the 
-second argument of type \<^verbatim>\<open>Result\<close> otherwise.\<close>
-definition result_or :: \<open>('a, 'f) result \<Rightarrow> ('a, 'e) result \<Rightarrow> ('s, ('a, 'e) result, 'abort, 'i, 'o) function_body\<close> where
-  \<open>result_or self e \<equiv> FunctionBody \<lbrakk>
-     match self {
-        Ok(v) \<Rightarrow> Ok(v),
-        Err(_) \<Rightarrow> e
-     } 
-  \<rbrakk>\<close>
-notation_nano_rust_function result_or ("or")
-
-definition result_or_pure :: \<open>('a, 'f) result \<Rightarrow> ('a, 'e) result \<Rightarrow> ('a, 'e) result\<close> where
-  \<open>result_or_pure v e \<equiv> case v of Ok(v) \<Rightarrow> Ok(v) | Err(_) \<Rightarrow> e\<close>
-
-lemma result_or_pure_simps[simp]:
-  shows \<open>result_or_pure (Ok v) f = Ok v\<close>
-    and \<open>result_or_pure (Err e) f = f\<close>
-  by (auto simp add: result_or_pure_def)
-
-definition result_or_contract :: 
-  \<open>('a, 'e) result \<Rightarrow> ('a, 'f) result \<Rightarrow> ('s::{sepalg}, ('a, 'f) result, 'abort) function_contract\<close>
-  where [crush_contracts]: \<open>result_or_contract res if_err \<equiv>
-    let pre = UNIV; post = \<lambda>r. \<langle>r = result_or_pure res if_err\<rangle>
-    in make_function_contract pre post\<close>
-ucincl_auto result_or_contract
-
-lemma result_or_spec [crush_specs]:
-  shows \<open>\<Gamma>; result_or res if_err \<Turnstile>\<^sub>F result_or_contract res if_err\<close>
-  by (crush_boot f: result_or_def contract: result_or_contract_def)
-     (crush_base simp add: result_or_pure_def split!: result.splits)
-
-text\<open>Maps a function to the \<^verbatim>\<open>Err\<close> constructor of the \<^verbatim>\<open>Result\<close> type.\<close>
-definition map_err :: \<open>('a, 'e) result \<Rightarrow> ('e \<Rightarrow> ('machine, 'f, 'abort, 'i, 'o) function_body) \<Rightarrow>
-    ('machine, ('a, 'f) result, 'abort, 'i, 'o) function_body\<close> where
-  \<open>map_err x f \<equiv> FunctionBody \<lbrakk>
-     match x {
-       Ok(a)  \<Rightarrow> Ok(a),
-       Err(e) \<Rightarrow> Err(f(e))
-     }
-  \<rbrakk>\<close>
-
-definition map_err_contract :: \<open>('a, 'e) result \<Rightarrow> ('e \<Rightarrow> 'f) \<Rightarrow> 
-('machine::sepalg, 'abort, 'i, 'o) striple_context \<Rightarrow>
-('e \<Rightarrow> ('machine, 'f, 'abort, 'i prompt, 'o prompt_output) function_body) \<Rightarrow>
-('machine, ('a, 'f) result, 'abort) function_contract\<close> where
-  [crush_contracts]: \<open>map_err_contract res pure_fun \<Gamma> rust_fun \<equiv>
-    let pre  = \<langle>\<forall> i. \<Gamma>; rust_fun i \<Turnstile>\<^sub>F lift_pure_to_contract (pure_fun i)\<rangle>;
-        post = \<lambda>r. \<langle>r = (case res of Err(e) \<Rightarrow> Err(pure_fun e) | Ok(k) \<Rightarrow> Ok(k))\<rangle>
-    in make_function_contract pre post\<close>
-ucincl_auto map_err_contract
-declare lift_pure_to_contract_def [crush_contracts]
-ucincl_auto lift_pure_to_contract
-
-lemma map_err_spec [crush_specs]:
-  shows \<open>\<Gamma>; map_err res rust_fun \<Turnstile>\<^sub>F map_err_contract res pure_fun \<Gamma> rust_fun\<close>
-proof (crush_boot f: map_err_def contract: map_err_contract_def, goal_cases)
-  case 1
-  note rust_fun_spec = this[THEN spec]
-  show ?case
-  proof (cases res)
-    case (Ok x1)
-    then show ?thesis by crush_base
-  next
-    case (Err x2)
-    then show ?thesis by (crush_base specs add: rust_fun_spec)
-  qed
-qed
-
-text\<open>Ok\<close>
-definition ok :: \<open>('v, 'e) result \<Rightarrow> ('s, 'v option, 'abort, 'i, 'o) function_body\<close> where
-  \<open>ok self \<equiv> FunctionBody \<lbrakk>
-     match self {
-       Ok(r) \<Rightarrow> Some(r),
-       Err(e) \<Rightarrow> None
-     }
-   \<rbrakk>\<close>
-
-definition ok_contract ::  \<open>('v, 'e) result \<Rightarrow> ('s::{sepalg}, 'v option, 'abort) function_contract\<close> where
-  [crush_contracts]: \<open>ok_contract res \<equiv>
-    let pre  = UNIV;
-        post = \<lambda>r. \<langle>r = (case res of Err(_) \<Rightarrow> None | Ok(k) \<Rightarrow> Some k)\<rangle>
-    in make_function_contract pre post\<close>
-ucincl_auto ok_contract
-
-lemma ok_spec [crush_specs]:
-  shows \<open>\<Gamma>; ok res \<Turnstile>\<^sub>F ok_contract res\<close>
-  apply (crush_boot f: ok_def contract: ok_contract_def)
-  apply (cases res)
-  apply crush_base
-  done
-
-definition err :: \<open>('v, 'e) result \<Rightarrow> ('s, 'e option, 'abort, 'i, 'o) function_body\<close> where
-  \<open>err self \<equiv> FunctionBody \<lbrakk>
-     match self {
-       Ok(r) \<Rightarrow> None,
-       Err(e) \<Rightarrow> Some(e)
-     }
-   \<rbrakk>\<close>
-
-definition err_contract ::  \<open>('v, 'e) result \<Rightarrow> ('s::{sepalg}, 'e option, 'abort) function_contract\<close> where
-  [crush_contracts]: \<open>err_contract res \<equiv>
-    let pre  = UNIV;
-        post = \<lambda>r. \<langle>r = (case res of Ok(_) \<Rightarrow> None | Err(k) \<Rightarrow> Some k)\<rangle>
-    in make_function_contract pre post\<close>
-ucincl_auto err_contract
-
-lemma err_spec [crush_specs]:
-  shows \<open>\<Gamma>; err res \<Turnstile>\<^sub>F err_contract res\<close>
-  apply (crush_boot f: err_def contract: err_contract_def)
-  apply (cases res)
-  apply crush_base
-  done
-
-definition result_unwrap_or :: \<open>('a, 'b) result \<Rightarrow> 'a \<Rightarrow> ('machine, 'a, 'abort, 'i prompt, 'o prompt_output) function_body\<close> where
-  \<open>result_unwrap_or res e \<equiv> FunctionBody \<lbrakk>
-     if let Ok(r) = res {
-       r
-     } else {
-       e
-     }
-   \<rbrakk>\<close>
-
-definition result_unwrap_or_contract ::  \<open>('a, 'b) result \<Rightarrow> 'a \<Rightarrow> ('s::{sepalg}, 'a, 'abort) function_contract\<close> where
-  [crush_contracts]: \<open>result_unwrap_or_contract res e \<equiv>
-    let pre  = UNIV;
-        post = \<lambda>r. \<langle>r = (case res of Ok(v) \<Rightarrow> v | Err(_) \<Rightarrow> e)\<rangle>
-    in make_function_contract pre post\<close>
-ucincl_auto result_unwrap_or_contract
-
-lemma result_unwrap_or_spec [crush_specs]:
-  shows \<open>\<Gamma>; result_unwrap_or res e \<Turnstile>\<^sub>F result_unwrap_or_contract res e\<close>
-  apply (crush_boot f: result_unwrap_or_def contract: result_unwrap_or_contract_def)
-  apply (cases res)
-  apply crush_base
-  done
+text\<open>Returns a mutable reference to the values inside the mutable \<^verbatim>\<open>Result\<close> type.\<close>
 
 context reference
 begin       
@@ -265,6 +59,307 @@ no_adhoc_overloading store_update_const \<rightleftharpoons> update_fun
 (*<*)
 end
 (*>*)
+
+subsection\<open>as_ref\<close>
+
+subsection\<open>cloned\<close>
+
+subsection\<open>copied\<close>
+
+subsection\<open>err\<close>
+
+text\<open>Converts a \<^verbatim>\<open>Result\<close> type into a \<^verbatim>\<open>Option\<close> type where only the err constructor 
+is kept while ok is discarded.\<close>
+
+definition result_err :: \<open>('v, 'e) result \<Rightarrow> ('s, 'e option, 'abort, 'i, 'o) function_body\<close> where
+  \<open>result_err self \<equiv> FunctionBody \<lbrakk>
+     match self {
+       Ok(r) \<Rightarrow> None,
+       Err(e) \<Rightarrow> Some(e)
+     }
+   \<rbrakk>\<close>
+
+definition result_err_contract ::  \<open>('v, 'e) result \<Rightarrow> ('s::{sepalg}, 'e option, 'abort) function_contract\<close> where
+  [crush_contracts]: \<open>result_err_contract res \<equiv>
+    let pre  = UNIV;
+        post = \<lambda>r. \<langle>r = (case res of Ok(_) \<Rightarrow> None | Err(k) \<Rightarrow> Some k)\<rangle>
+    in make_function_contract pre post\<close>
+ucincl_auto result_err_contract
+
+lemma result_err_spec [crush_specs]:
+  shows \<open>\<Gamma>; result_err res \<Turnstile>\<^sub>F result_err_contract res\<close>
+  apply (crush_boot f: result_err_def contract: result_err_contract_def)
+  apply (cases res)
+  apply crush_base
+  done
+
+subsection\<open>expect\<close>
+
+text\<open>Returns \<^verbatim>\<open>x\<close> if the element of \<^verbatim>\<open>Result\<close> type is of the form \<^verbatim>\<open>Ok x\<close>. Panics otherwise with
+the defined error message.\<close>
+
+definition result_expect :: \<open>('v,'e) result \<Rightarrow> String.literal \<Rightarrow> ('s, 'v, 'abort, 'i, 'o) function_body\<close> where
+  \<open>result_expect self msg \<equiv> FunctionBody \<lbrakk>
+      match self {
+        Ok(v) \<Rightarrow> v,
+        Err(_) \<Rightarrow> panic!(msg) 
+      }
+  \<rbrakk>\<close>
+adhoc_overloading expect \<rightleftharpoons> result_expect
+
+definition result_expect_contract :: 
+  \<open>('a, 'e) result \<Rightarrow> 'a \<Rightarrow> ('s::{sepalg}, 'a, 'abort) function_contract\<close>
+  where [crush_contracts]: \<open>result_expect_contract self v \<equiv>
+    let pre = \<langle>self = Ok v\<rangle>; post = \<lambda>r. \<langle>r = v\<rangle>
+    in make_function_contract pre post\<close>
+ucincl_auto result_expect_contract
+
+lemma result_expect_spec [crush_specs]:
+  shows \<open>\<Gamma>; result_expect res m \<Turnstile>\<^sub>F result_expect_contract res v\<close>
+  by (crush_boot f: result_expect_def contract: result_expect_contract_def)
+     (crush_base split!: result.splits)
+
+subsection\<open>expect_err\<close>
+
+subsection\<open>flatten\<close>
+
+subsection\<open>inspect\<close>
+
+subsection\<open>inspect_err\<close>
+
+subsection\<open>into_err\<close>
+
+subsection\<open>into_ok\<close>
+
+subsection\<open>is_err\<close>
+
+text\<open>Tests whether an element of \<^verbatim>\<open>Result\<close> type is the \<^verbatim>\<open>Err\<close> constructor:\<close>
+
+definition urust_func_result_is_err :: \<open>('v,'e) result \<Rightarrow> ('s, bool, 'abort, 'i, 'o) function_body\<close> where
+  \<open>urust_func_result_is_err self \<equiv> FunctionBody \<lbrakk>
+     match self {
+       Ok(_) \<Rightarrow> False,
+       Err(_) \<Rightarrow> True
+     }
+  \<rbrakk>\<close>
+
+definition result_is_err_contract :: 
+  \<open>('a, 'e) result \<Rightarrow> ('s::{sepalg}, bool, 'abort) function_contract\<close>
+  where [crush_contracts]: \<open>result_is_err_contract res \<equiv>
+    let pre = UNIV; post = \<lambda>r. \<langle>r = result_is_err res\<rangle>
+    in make_function_contract pre post\<close>
+ucincl_auto result_is_err_contract
+
+lemma result_is_err_spec [crush_specs]:
+  shows \<open>\<Gamma>; urust_func_result_is_err res \<Turnstile>\<^sub>F result_is_err_contract res\<close>
+  by (crush_boot f: urust_func_result_is_err_def contract: result_is_err_contract_def)
+     (crush_base simp add: result_is_err_def split!: result.splits)
+
+subsection\<open>is_err_and\<close>
+
+subsection\<open>is_ok\<close>
+
+text\<open>Tests whether an element of \<^verbatim>\<open>Result\<close> type is the \<^verbatim>\<open>Ok\<close> constructor:\<close>
+
+definition urust_func_result_is_ok :: \<open>('v,'e) result \<Rightarrow> ('s, bool, 'abort, 'i, 'o) function_body\<close> where
+  \<open>urust_func_result_is_ok self \<equiv> FunctionBody \<lbrakk>
+     match self {
+       Ok(_) \<Rightarrow> True,
+       Err(_) \<Rightarrow> False
+     }
+  \<rbrakk>\<close>
+
+definition result_is_ok_contract :: 
+  \<open>('a, 'e) result \<Rightarrow> ('s::{sepalg}, bool, 'abort) function_contract\<close>
+  where [crush_contracts]: \<open>result_is_ok_contract res \<equiv>
+    let pre = UNIV; post = \<lambda>r. \<langle>r = result_is_ok res\<rangle>
+    in make_function_contract pre post\<close>
+ucincl_auto result_is_ok_contract
+
+lemma result_is_ok_spec [crush_specs]:
+  shows \<open>\<Gamma>; urust_func_result_is_ok res \<Turnstile>\<^sub>F result_is_ok_contract res\<close>
+  by (crush_boot f: urust_func_result_is_ok_def contract: result_is_ok_contract_def)
+     (crush_base simp add: result_is_ok_def split!: result.splits)
+
+subsection\<open>is_ok_and\<close>
+
+subsection\<open>iter\<close>
+
+subsection\<open>iter_mut\<close>
+
+subsection\<open>map\<close>
+
+subsection\<open>map_err\<close>
+
+text\<open>Maps a function to the \<^verbatim>\<open>Err\<close> constructor of the \<^verbatim>\<open>Result\<close> type.\<close>
+
+definition result_map_err :: \<open>('a, 'e) result \<Rightarrow> ('e \<Rightarrow> ('machine, 'f, 'abort, 'i, 'o) function_body) \<Rightarrow>
+    ('machine, ('a, 'f) result, 'abort, 'i, 'o) function_body\<close> where
+  \<open>result_map_err x f \<equiv> FunctionBody \<lbrakk>
+     match x {
+       Ok(a)  \<Rightarrow> Ok(a),
+       Err(e) \<Rightarrow> Err(f(e))
+     }
+  \<rbrakk>\<close>
+
+definition result_map_err_contract :: \<open>('a, 'e) result \<Rightarrow> ('e \<Rightarrow> 'f) \<Rightarrow> 
+('machine::sepalg, 'abort, 'i, 'o) striple_context \<Rightarrow>
+('e \<Rightarrow> ('machine, 'f, 'abort, 'i prompt, 'o prompt_output) function_body) \<Rightarrow>
+('machine, ('a, 'f) result, 'abort) function_contract\<close> where
+  [crush_contracts]: \<open>result_map_err_contract res pure_fun \<Gamma> rust_fun \<equiv>
+    let pre  = \<langle>\<forall> i. \<Gamma>; rust_fun i \<Turnstile>\<^sub>F lift_pure_to_contract (pure_fun i)\<rangle>;
+        post = \<lambda>r. \<langle>r = (case res of Err(e) \<Rightarrow> Err(pure_fun e) | Ok(k) \<Rightarrow> Ok(k))\<rangle>
+    in make_function_contract pre post\<close>
+ucincl_auto result_map_err_contract
+declare lift_pure_to_contract_def [crush_contracts]
+ucincl_auto lift_pure_to_contract
+
+lemma result_map_err_spec [crush_specs]:
+  shows \<open>\<Gamma>; result_map_err res rust_fun \<Turnstile>\<^sub>F result_map_err_contract res pure_fun \<Gamma> rust_fun\<close>
+proof (crush_boot f: result_map_err_def contract: result_map_err_contract_def, goal_cases)
+  case 1
+  note rust_fun_spec = this[THEN spec]
+  show ?case
+  proof (cases res)
+    case (Ok x1)
+    then show ?thesis by crush_base
+  next
+    case (Err x2)
+    then show ?thesis by (crush_base specs add: rust_fun_spec)
+  qed
+qed
+
+subsection\<open>map_or\<close>
+
+subsection\<open>map_or_default\<close>
+
+subsection\<open>map_or_else\<close>
+
+subsection\<open>ok\<close>
+
+text\<open>Converts a \<^verbatim>\<open>Result\<close> type into a \<^verbatim>\<open>Option\<close> type where only the ok constructor 
+is kept while err is discarded.\<close>
+
+definition result_ok :: \<open>('v, 'e) result \<Rightarrow> ('s, 'v option, 'abort, 'i, 'o) function_body\<close> where
+  \<open>result_ok self \<equiv> FunctionBody \<lbrakk>
+     match self {
+       Ok(r) \<Rightarrow> Some(r),
+       Err(e) \<Rightarrow> None
+     }
+   \<rbrakk>\<close>
+
+definition result_ok_contract ::  \<open>('v, 'e) result \<Rightarrow> ('s::{sepalg}, 'v option, 'abort) function_contract\<close> where
+  [crush_contracts]: \<open>result_ok_contract res \<equiv>
+    let pre  = UNIV;
+        post = \<lambda>r. \<langle>r = (case res of Err(_) \<Rightarrow> None | Ok(k) \<Rightarrow> Some k)\<rangle>
+    in make_function_contract pre post\<close>
+ucincl_auto result_ok_contract
+
+lemma result_ok_spec [crush_specs]:
+  shows \<open>\<Gamma>; result_ok res \<Turnstile>\<^sub>F result_ok_contract res\<close>
+  apply (crush_boot f: result_ok_def contract: result_ok_contract_def)
+  apply (cases res)
+  apply crush_base
+  done
+
+subsection\<open>or\<close>
+
+text\<open>Returns first argument of type \<^verbatim>\<open>Result\<close> if it is the \<^verbatim>\<open>Ok\<close> constructor, returns the 
+second argument of type \<^verbatim>\<open>Result\<close> otherwise.\<close>
+
+definition result_or :: \<open>('a, 'f) result \<Rightarrow> ('a, 'e) result \<Rightarrow> ('s, ('a, 'e) result, 'abort, 'i, 'o) function_body\<close> where
+  \<open>result_or self e \<equiv> FunctionBody \<lbrakk>
+     match self {
+        Ok(v) \<Rightarrow> Ok(v),
+        Err(_) \<Rightarrow> e
+     } 
+  \<rbrakk>\<close>
+notation_nano_rust_function result_or ("or")
+
+definition result_or_pure :: \<open>('a, 'f) result \<Rightarrow> ('a, 'e) result \<Rightarrow> ('a, 'e) result\<close> where
+  \<open>result_or_pure v e \<equiv> case v of Ok(v) \<Rightarrow> Ok(v) | Err(_) \<Rightarrow> e\<close>
+
+lemma result_or_pure_simps[simp]:
+  shows \<open>result_or_pure (Ok v) f = Ok v\<close>
+    and \<open>result_or_pure (Err e) f = f\<close>
+  by (auto simp add: result_or_pure_def)
+
+definition result_or_contract :: 
+  \<open>('a, 'e) result \<Rightarrow> ('a, 'f) result \<Rightarrow> ('s::{sepalg}, ('a, 'f) result, 'abort) function_contract\<close>
+  where [crush_contracts]: \<open>result_or_contract res if_err \<equiv>
+    let pre = UNIV; post = \<lambda>r. \<langle>r = result_or_pure res if_err\<rangle>
+    in make_function_contract pre post\<close>
+ucincl_auto result_or_contract
+
+lemma result_or_spec [crush_specs]:
+  shows \<open>\<Gamma>; result_or res if_err \<Turnstile>\<^sub>F result_or_contract res if_err\<close>
+  by (crush_boot f: result_or_def contract: result_or_contract_def)
+     (crush_base simp add: result_or_pure_def split!: result.splits)
+
+subsection\<open>or_else\<close>
+
+subsection\<open>transpose\<close>
+
+subsection\<open>unwrap\<close>
+
+text\<open>Returns \<^verbatim>\<open>x\<close> if the element of \<^verbatim>\<open>Result\<close> type is of the form \<^verbatim>\<open>Ok x\<close>.  Panics otherwise.\<close>
+
+definition result_unwrap :: \<open>('v,'e) result \<Rightarrow> ('s, 'v, 'abort, 'i, 'o) function_body\<close> where
+  \<open>result_unwrap self \<equiv> FunctionBody \<lbrakk>
+      self.expect("result_unwrap")
+  \<rbrakk>\<close>
+adhoc_overloading unwrap \<rightleftharpoons> result_unwrap
+
+definition result_unwrap_contract :: 
+  \<open>('a, 'e) result \<Rightarrow> 'a \<Rightarrow> ('s::{sepalg}, 'a, 'abort) function_contract\<close>
+  where [crush_contracts]: \<open>result_unwrap_contract self v \<equiv>
+    let pre = \<langle>self = Ok v\<rangle>; post = \<lambda>r. \<langle>r = v\<rangle>
+    in make_function_contract pre post\<close>
+ucincl_auto result_unwrap_contract
+
+lemma result_unwrap_spec [crush_specs]:
+  shows \<open>\<Gamma>; result_unwrap res \<Turnstile>\<^sub>F result_unwrap_contract res v\<close>
+  by (crush_boot f: result_unwrap_def contract: result_unwrap_contract_def)
+     (crush_base split!: result.splits)
+
+subsection\<open>unwrap_err\<close>
+
+subsection\<open>unwrap_err_unchecked\<close>
+
+subsection\<open>unrwrap_or\<close>
+
+text\<open>Returns the \<^verbatim>\<open>Ok\<close> constructor of \<^verbatim>\<open>Result\<close> or the provided default, 
+dependant on the content of \<^verbatim>\<open>Result\<close>.\<close>
+
+definition result_unwrap_or :: \<open>('a, 'b) result \<Rightarrow> 'a \<Rightarrow> ('machine, 'a, 'abort, 'i prompt, 'o prompt_output) function_body\<close> where
+  \<open>result_unwrap_or res e \<equiv> FunctionBody \<lbrakk>
+     match res {
+      Ok(r) \<Rightarrow> r,
+      Err(_) \<Rightarrow> e
+    }
+   \<rbrakk>\<close>
+
+definition result_unwrap_or_contract ::  \<open>('a, 'b) result \<Rightarrow> 'a \<Rightarrow> ('s::{sepalg}, 'a, 'abort) function_contract\<close> where
+  [crush_contracts]: \<open>result_unwrap_or_contract res e \<equiv>
+    let pre  = UNIV;
+        post = \<lambda>r. \<langle>r = (case res of Ok(v) \<Rightarrow> v | Err(_) \<Rightarrow> e)\<rangle>
+    in make_function_contract pre post\<close>
+ucincl_auto result_unwrap_or_contract
+
+lemma result_unwrap_or_spec [crush_specs]:
+  shows \<open>\<Gamma>; result_unwrap_or res e \<Turnstile>\<^sub>F result_unwrap_or_contract res e\<close>
+  apply (crush_boot f: result_unwrap_or_def contract: result_unwrap_or_contract_def)
+  apply (cases res)
+  apply crush_base
+  done
+
+subsection\<open>unwrap_or_default\<close>
+
+subsection\<open>unwrap_or_else\<close>
+
+subsection\<open>unwrap_unchecked\<close>
+
+section\<open>Debug\<close>
 
 instantiation result :: (generate_debug,generate_debug)generate_debug
 begin
